feat(CFG): Correctnesses!

Cslib/Analysis/Dataflow/Kildall.lean
@@ -11,21 +11,28 @@ import Mathlib.Data.DFinsupp.WellFounded
 /-!
 # Forward Worklist dataflow algorithm
 
-Implementation of Kildall's worklist algorithm for solving dataflow equations,
-as described in @Kildall73.
+Implementation of Kildall's worklist algorithm for solving dataflow equations, as described in
+@Kildall73. Correctness follows an argument similar to the one found in @Nielson99, with a proof
+technique borrowed from @LaSpina25.
 
 ## Main definitions
 
-- `DFState` represents the result of a dataflow analysis algorithm, a mapping
-  between CFG nodes and abstract states
+- `DFState` represents the result of a dataflow analysis algorithm, a mapping between CFG nodes and
+  abstract states.
+- Definitions of correctness (soundness + completeness) for the analysis result, as `Fixpoint`s over
+  the analysis result `ρ`.
+-
 
 ## Main theorems
 
 - Termination of the worklist algorithm
+- Correctness of the algorithm : computation of a postfixpoint.
+- Correctness of the algorithm : computation of a fixpoint in the monotone transfer case.
 
 ## References
 
 * [G. Kildall, *A Unified Approach to Global Program Optimization*][Kildall73]
+* [F. Nielson, H.R. Nielson, C. Hankin, *Principles of Program Analysis*][Nielson99]
 * [R. LaSpina, *Formal Verification of WTO-based Dataflow Solvers*][LaSpina25]
 -/
 
@@ -40,7 +47,7 @@ namespace DFState
 variable {L : Type} [SemilatticeSup L]
 
 /-- The empty dataflow result, a function mapping every node to `⊥`. -/
-def empty {g : CFG Node Edge} [Bot L] : DFState g L := fun _ => ⊥
+def empty {g : CFG Node Edge} [OrderBot L] : DFState g L := fun _ => ⊥
 
 /-- Update `ρ`'s value at node `n`, to new value `v`. -/
 def update {g : CFG Node Edge} (ρ : DFState g L) (n : NodeOf g) (v : L) : DFState g L :=
@@ -56,7 +63,7 @@ end DFState
 
 section Kildall
 
-variable {L : Type} [SemilatticeSup L] [DecidableEq L] [Bot L]
+variable {L : Type} [SemilatticeSup L] [DecidableEq L] [OrderBot L]
 
 /-- if there's no ascending chains in `L`, there are no ascending chains in `DFState g L` either -/
 instance {g : CFG Node Edge} [WellFoundedGT L] : WellFoundedGT (DFState g L) :=
@@ -70,35 +77,209 @@ local instance {g : CFG Node Edge} [WellFoundedGT L] : WellFoundedRelation (DFSt
 -- abstract shape of transfer function
 abbrev Transfer (α L : Type) := α -> L -> L
 
-def joinPred (g : CFG Node Edge) (eT : Transfer Edge L) (s : DFState g L) (n : NodeOf g) : L :=
-  (g.inEdges n).foldl (fun acc e =>
-    let src : NodeOf g := g.srcOf e
-    acc ⊔ eT e (s src)
-  ) ⊥
+def joinPred (g : CFG Node Edge) (eT : Transfer Edge L) (init : L) (ρ : DFState g L)
+    (n : NodeOf g) : L :=
+  (g.inEdges n).foldl (fun acc (e : EdgeOf g) =>
+    acc ⊔ eT e (ρ (g.srcOf e))
+  ) (if n.val = g.entry then init else ⊥)
 
 /-- Kildall's worklist algorithm, propagating updates to the worklist based on new information.
     The termination proof uses wellfoundedness of · < · on `L`, i.e. the fact that the lattice
     is of finite height. -/
 def kildall [WellFoundedGT L]
     (g : CFG Node Edge) (nT : Transfer Node L) (eT : Transfer Edge L)
-    (init : L) (acc : DFState g L := DFState.empty)
+    (init : L) (ρ : DFState g L := DFState.empty)
     (wl : List (NodeOf g) := g.nodesOf) : DFState g L :=
   match wl with
-  | [] => acc
+  | [] => ρ
   | n :: rest =>
-      let newIn := joinPred g eT acc n
-      let newOut := (acc n) ⊔ (nT n newIn)
-      if _h : newOut = (acc n) then
-        kildall g nT eT init acc rest
+      let newIn := joinPred g eT init ρ n
+      let newOut := (ρ n) ⊔ (nT n newIn)
+      if _h : newOut = (ρ n) then
+        kildall g nT eT init ρ rest
       else
-        let acc' := DFState.update acc n newOut
+        let ρ' := DFState.update ρ n newOut
         let wl' := rest ++ g.succOf n
-        kildall g nT eT init acc' wl'
-termination_by (acc, wl.length)
+        kildall g nT eT init ρ' wl'
+termination_by (ρ, wl.length)
 decreasing_by
-  · exact Prod.Lex.right acc (by simp)
+  · exact Prod.Lex.right ρ (by simp)
   · refine Prod.Lex.left _ _ ?_
     apply DFState.lt_update
     apply le_sup_left.lt_of_ne; grind
 
 end Kildall
+
+section Properties
+
+variable {L : Type} [SemilatticeSup L] [WellFoundedGT L] [OrderBot L]
+
+omit [WellFoundedGT L] in
+/-- Updating the abstract state at node `m` doesn't impact the incoming state at node `n` if `m` is
+    not a predecessor of `n`. -/
+lemma joinPred_neq_of_nonpred (g : CFG Node Edge) (eT : Transfer Edge L) (init : L)
+    (ρ : DFState g L) (n m : NodeOf g) (v : L) (hm : n ∉ g.succOf m) :
+    joinPred g eT init (ρ.update m v) n = joinPred g eT init ρ n := by
+  simp only [joinPred]
+  apply List.foldl_ext
+  intro acc e he
+  simp only [DFState.update]
+  split
+  case isFalse hneq => rfl
+  case isTrue heq =>
+    exfalso
+    apply hm
+    simp only [CFG.succOf, CFG.nodesOf, List.mem_filter, List.mem_attach, List.any_eq_true,
+      decide_eq_true_eq, Subtype.exists, true_and]
+    use e, e.property
+
+omit [WellFoundedGT L] in
+/-- Incoming states are monotone when every edge transfer is monotone. -/
+lemma monotone_joinPred (g : CFG Node Edge) (eT : Transfer Edge L) (init : L)
+    (heT : ∀ e, Monotone (eT e)) : Monotone (joinPred g eT init) := by
+  intro ρ₁ ρ₂ hle
+  apply Pi.le_def.2
+  intro n
+  simp only [joinPred]
+  suffices ∀ init₁ init₂, init₁ <= init₂ →
+    List.foldl _ init₁ (g.inEdges n) ≤ List.foldl _ init₂ (g.inEdges n) by
+    apply Std.IsPreorder.le_refl _ |> this _ _
+  induction g.inEdges n with
+  | nil => simp
+  | cons e t ih =>
+    intros i₁ i₂ hlei
+    simp only [List.foldl_cons]
+    refine sup_le_sup hlei ?_ |> ih _ _
+    exact heT e (hle _)
+
+/- To prove properties on this algorithm, we adapt a technique from @LaSpina25 to exploit the
+inductive structure of the algorithm's execution. -/
+
+/-- The result of the worklist algorithm satisfies any invariant preserved through the
+    algorithm's run. -/
+lemma kildall_invariant [DecidableEq L]
+    (g : CFG Node Edge) (nT : Transfer Node L) (eT : Transfer Edge L)
+    (init : L) (ρ : DFState g L) (wl : List (NodeOf g))
+    (P : DFState g L → List (NodeOf g) → Prop)
+    (hinit : P ρ wl)
+    (hstep_same : ∀ {ρ n rest}, P ρ (n :: rest) →
+      let newOut := ρ n ⊔ nT n (joinPred g eT init ρ n)
+      newOut = ρ n →
+        P ρ rest)
+    (hstep_changed : ∀ {ρ n rest}, P ρ (n :: rest) →
+      let newOut := ρ n ⊔ nT n (joinPred g eT init ρ n)
+      newOut ≠ ρ n →
+        P (ρ.update n newOut) (rest ++ g.succOf n)) :
+      P (kildall g nT eT init ρ wl) [] := by
+  induction ρ, wl using kildall.induct g nT eT init with
+  | case1 o => simpa [kildall]
+  | case2 acc n rest nin nout heq ih =>
+      simp only [kildall, dite_eq_ite]
+      rw [if_pos heq]
+      exact ih (hstep_same hinit heq)
+  | case3 acc n r nin nout hnout acc' wl' ih =>
+      simp only [kildall, dite_eq_ite]
+      rw [if_neg hnout]
+      exact ih (hstep_changed hinit hnout)
+
+/-- An analysis result `ρ` on `g` is a postfixpoint if, at every node of `g`, computing the
+    transfers of the incoming facts remains within the outgoing facts. -/
+def ForwardPostFixpoint
+    (g : CFG Node Edge) (nT : Transfer Node L) (eT : Transfer Edge L) (init : L)
+    (ρ : DFState g L) (wl : List (NodeOf g)) : Prop :=
+  ∀ n ∉ wl, nT n (joinPred g eT init ρ n) ≤ ρ n
+
+/-- An analysis result `ρ` on `g` is a fixpoint if, at every node of `g`, the `ForwardPostFixpoint`
+    bound is tight. -/
+def ForwardFixpoint
+    (g : CFG Node Edge) (nT : Transfer Node L) (eT : Transfer Edge L) (init : L)
+    (ρ : DFState g L) (wl : List (NodeOf g)) : Prop :=
+  ∀ n ∉ wl, nT n (joinPred g eT init ρ n) = ρ n
+
+/-- The result of the worklist algorithm is a `ForwardPostfixpoint`. -/
+theorem kildall_forwardPostFixpoint [DecidableEq L] (g : CFG Node Edge)
+    (nT : Transfer Node L) (eT : Transfer Edge L) (init : L) (ρ : DFState g L)
+    (wl : List (NodeOf g))
+    (hinv0 : ∀ m : NodeOf g, m ∉ wl → nT m (joinPred g eT init ρ m) ≤ ρ m) :
+    let res := kildall g nT eT init ρ wl
+    ForwardPostFixpoint g nT eT init res [] := by
+  refine kildall_invariant g nT eT init ρ wl (ForwardPostFixpoint g nT eT init) ?_ ?_ ?_
+  · exact hinv0
+  · intro ρ n rest hfp newOut heq m hm
+    by_cases hmn : m = n
+    · subst m
+      exact le_sup_right.trans_eq heq
+    · exact hfp m (by simp_all)
+  · intro ρ n rest hfp newOut hnout m hm
+    have hsucc : m ∉ g.succOf n := fun hin => (List.mem_append_right _ hin) |> hm
+    rw [joinPred_neq_of_nonpred g eT init ρ m n newOut hsucc, DFState.update]
+    split -- m ?= n
+    case isTrue heq =>
+      grind [le_sup_right]
+    case isFalse hneq =>
+      apply hfp; grind
+
+/-- An analysis result `ρ` on `g` is a prefixpoint if every outgoing fact remains within the
+    result of transferring its incoming facts. -/
+def ForwardPreFixpoint (g : CFG Node Edge) (nT : Transfer Node L) (eT : Transfer Edge L) (init : L)
+    (ρ : DFState g L) : Prop :=
+  ∀ n, ρ n ≤ nT n (joinPred g eT init ρ n)
+
+/-- The worklist algorithm preserves forward pre-fixpoints when all transfers are monotone. -/
+lemma kildall_forwardPreFixpoint [DecidableEq L] (g : CFG Node Edge)
+    (nT : Transfer Node L) (hnT : ∀ n, Monotone (nT n))
+    (eT : Transfer Edge L) (heT : ∀ e, Monotone (eT e))
+    (init : L) (ρ : DFState g L) (wl : List (NodeOf g))
+    (hinv0 : ForwardPreFixpoint g nT eT init ρ) :
+    let res := kildall g nT eT init ρ wl
+    ForwardPreFixpoint g nT eT init res := by
+  refine kildall_invariant g nT eT init ρ wl
+    (fun ρ _ => ForwardPreFixpoint g nT eT init ρ) hinv0 ?_ ?_
+  · exact fun hfp _ => hfp
+  · intro ρ n rest hfp newOut hnout m
+    have hle : ρ ≤ ρ.update n newOut := by
+      intro k
+      simp only [DFState.update]
+      split <;> grind [le_refl, le_sup_left]
+    have htransfer : nT m (joinPred g eT init ρ m) ≤
+        nT m (joinPred g eT init (ρ.update n newOut) m) :=
+      hnT m (monotone_joinPred g eT init heT hle m)
+    grind [DFState.update, sup_le, hfp m]
+
+/-- If the transfer functions are monotone, the result of the worklist algorithm is a
+    `ForwardFixpoint`. -/
+theorem kildall_forwardFixpoint [DecidableEq L] (g : CFG Node Edge)
+    (nT : Transfer Node L) (hnT : ∀ n, Monotone (nT n))
+    (eT : Transfer Edge L) (heT : ∀ e, Monotone (eT e))
+    (init : L) (ρ : DFState g L) (wl : List (NodeOf g))
+    (hpost0 : ∀ m ∉ wl, nT m (joinPred g eT init ρ m) ≤ ρ m)
+    (hpre0 : ForwardPreFixpoint g nT eT init ρ) :
+    let res := kildall g nT eT init ρ wl
+    ForwardFixpoint g nT eT init res [] := by
+  intro res
+  have hpost : ForwardPostFixpoint g nT eT init res [] :=
+    kildall_forwardPostFixpoint g nT eT init ρ wl hpost0
+  have hpre : ForwardPreFixpoint g nT eT init res :=
+    kildall_forwardPreFixpoint g nT hnT eT heT init ρ wl hpre0
+  intro n hn
+  exact le_antisymm (hpost n hn) (hpre n)
+
+/-- Final theorem: the result of a full run of the algorithm with the default arguments is the least
+    fixpoint of the equations induced by the transfer functions and the initial state. -/
+theorem kildall_correct [DecidableEq L] (g : CFG Node Edge)
+    (nT : Transfer Node L) (hnT : ∀ n, Monotone (nT n))
+    (eT : Transfer Edge L) (heT : ∀ e, Monotone (eT e))
+    (init : L) :
+    let res := kildall g nT eT init
+    ForwardFixpoint g nT eT init res [] := by
+  apply kildall_forwardFixpoint g nT hnT eT heT init DFState.empty g.nodesOf
+  case hpost0 => -- ≤
+    -- `∀ m ∉ g.nodesOf, ...`
+    -- since every `m` is in `g.nodesOf` this is vacuously true
+    grind [CFG.nodesOf]
+  case hpre0 => -- ≥
+    -- `∀ m ∈ g.nodesOf, DFState.empty m ≤ ...`
+    -- since `DFState.empty` is `λ _. ⊥`, it's ≤ anything, thanks to `OrderBot`.
+    simp [ForwardPreFixpoint, DFState.empty]
+
+end Properties
